src/request_response/DY.Example.RequestResponse.Protocol.Total.Proof.fst
@@ -13,9 +13,9 @@ open DY.Example.RequestResponse.Protocol.Stateful
 val crypto_usages_protocol: crypto_usages
 instance crypto_usages_protocol = default_crypto_usages
 
-val pkenc_pred_list_protocol: list (string & pkenc_crypto_predicate)
-let pkenc_pred_list_protocol = [
-  pkenc_crypto_predicates_communication_layer_and_tag
+val pke_pred_list_protocol: list (string & pke_crypto_predicate)
+let pke_pred_list_protocol = [
+  pke_crypto_predicates_communication_layer_and_tag
 ]
 
 val sign_pred_list_protocol: list (string & sign_crypto_predicate)
@@ -33,7 +33,7 @@ val crypto_predicates_protocol: crypto_predicates
 let crypto_predicates_protocol = {
   default_crypto_predicates with
 
-  pkenc_pred = mk_pkenc_predicate pkenc_pred_list_protocol;
+  pke_pred = mk_pke_predicate pke_pred_list_protocol;
 
   sign_pred = mk_sign_predicate sign_pred_list_protocol;
 
@@ -47,18 +47,18 @@ instance crypto_invariants_protocol: crypto_invariants = {
 }
 
 #push-options "--ifuel 0 --fuel 1"
-val pkenc_pred_has_all_pkenc_preds: 
+val pke_pred_has_all_pke_preds: 
   unit ->
   Lemma
   (ensures
-    norm [delta_only [`%pkenc_pred_list_protocol; `%for_allP]; iota; zeta] (
-      for_allP has_pkenc_predicate pkenc_pred_list_protocol
+    norm [delta_only [`%pke_pred_list_protocol; `%for_allP]; iota; zeta] (
+      for_allP has_pke_predicate pke_pred_list_protocol
     )
   )
-let pkenc_pred_has_all_pkenc_preds () =
-  assert_norm(List.Tot.no_repeats_p (List.Tot.map fst (pkenc_pred_list_protocol)));
-  mk_pkenc_predicate_correct pkenc_pred_list_protocol;
-  norm_spec [delta_only [`%pkenc_pred_list_protocol; `%for_allP]; iota; zeta] (for_allP has_pkenc_predicate pkenc_pred_list_protocol);
+let pke_pred_has_all_pke_preds () =
+  assert_norm(List.Tot.no_repeats_p (List.Tot.map fst (pke_pred_list_protocol)));
+  mk_pke_predicate_correct pke_pred_list_protocol;
+  norm_spec [delta_only [`%pke_pred_list_protocol; `%for_allP]; iota; zeta] (for_allP has_pke_predicate pke_pred_list_protocol);
   ()
 
 val sign_pred_has_all_sign_preds:
@@ -92,46 +92,7 @@ let aead_pred_has_all_aead_preds () =
 
 val protocol_crypto_invariants_has_communication_layer_crypto_predicates: squash has_communication_layer_reqres_crypto_predicates
 let protocol_crypto_invariants_has_communication_layer_crypto_predicates =
-  pkenc_pred_has_all_pkenc_preds ();
+  pke_pred_has_all_pke_preds ();
   sign_pred_has_all_sign_preds ();
   aead_pred_has_all_aead_preds ();
   ()
-
-(*** Proofs ***)
-
-val compute_message_proof:
-  tr:trace ->
-  client:principal -> server:principal ->
-  nonce:bytes ->
-  Lemma
-  (requires
-    is_knowable_by (join (principal_label client) (principal_label server)) tr nonce
-  )
-  (ensures
-    is_knowable_by (join (principal_label client) (principal_label server)) tr (compute_message client nonce)
-  )
-let compute_message_proof tr client server nonce =
-  let req:request = { client; nonce } in
-  serialize_wf_lemma request (is_knowable_by (join (principal_label client) (principal_label server)) tr) req;
-  ()
-
-val decode_message_proof:
-  tr:trace ->
-  server:principal ->
-  req_bytes:bytes -> req_label:label ->
-  Lemma
-  (requires
-    is_knowable_by req_label tr req_bytes
-  )
-  (ensures (
-    match decode_message req_bytes with
-    | None -> True
-    | Some {client=client'; nonce} -> is_knowable_by req_label tr nonce
-  ))
-let decode_message_proof tr server req_bytes req_label =
-  match decode_message req_bytes with
-  | None -> ()
-  | Some {client; nonce} -> (    
-    parse_wf_lemma request (is_knowable_by req_label tr) req_bytes;
-    ()
-  )
