src/single_conf_message/DY.Example.SingleConfMessage.Protocol.Stateful.Proof.fst
@@ -14,15 +14,14 @@ open DY.Example.SingleConfMessage.Protocol.Stateful
 let state_predicate_protocol: local_state_predicate single_message_state = {
   pred = (fun tr prin state_id st ->
     match st with
-    | SenderState receiver secret -> (
+    | SenderState receiver msg -> (
       let sender = prin in
-      get_label tr secret == join (principal_label sender) (principal_label receiver) /\
-      is_knowable_by (join (principal_label sender) (principal_label receiver)) tr secret
+      get_label tr msg.secret == join (principal_label sender) (principal_label receiver) /\
+      is_knowable_by (join (principal_label sender) (principal_label receiver)) tr msg.secret
     )
-    | ReceiverState secret payload -> (
+    | ReceiverState msg -> (
       let receiver = prin in
-      is_knowable_by (principal_label receiver) tr secret /\
-      is_knowable_by (principal_label receiver) tr payload
+      is_knowable_by (principal_label receiver) tr msg.secret
     )
   );
   pred_later = (fun tr1 tr2 prin state_id st -> ());
@@ -32,12 +31,11 @@ let state_predicate_protocol: local_state_predicate single_message_state = {
 let event_predicate_protocol: event_predicate single_message_event =
   fun tr prin e ->
     match e with
-    | SenderSendMsg sender receiver secret -> True
-    | ReceiverReceivedMsg receiver secret payload -> (
+    | SenderSendMsg sender receiver msg -> True
+    | ReceiverReceivedMsg receiver msg -> (
       exists sender.
-        is_knowable_by (join (principal_label sender) (principal_label receiver)) tr secret /\
-        is_knowable_by (join (principal_label sender) (principal_label receiver)) tr payload /\
-        event_triggered tr receiver (CommConfReceiveMsg receiver payload)
+        is_knowable_by (join (principal_label sender) (principal_label receiver)) tr msg.secret /\
+        event_triggered tr receiver (CommConfReceiveMsg receiver (serialize single_message msg))
     )
 
 let all_sessions = [
@@ -52,27 +50,23 @@ let all_sessions = [
 // If you don't need them you can just initialize them with
 // `default_comm_higher_layer_event_preds`.
 #push-options "--fuel 0 --ifuel 2"
-val comm_layer_event_preds: comm_higher_layer_event_preds
+val comm_layer_event_preds: comm_higher_layer_event_preds single_message
 let comm_layer_event_preds = {
-  default_comm_higher_layer_event_preds with
-  send_conf = (fun tr sender receiver payload -> 
-    match decode_message payload with
-    | None -> False
-    | Some {secret} -> (
-      event_triggered tr sender (SenderSendMsg sender receiver secret) /\
+  default_comm_higher_layer_event_preds single_message with
+  send_conf = (fun tr sender receiver (msg:single_message) -> 
+    event_triggered tr sender (SenderSendMsg sender receiver msg) /\
 
-      // The user of the communication layer can
-      // also use this function to demand specific
-      // labels from parts of the payload. These
-      // labels can then be used on the receiver
-      // side. With the following requirement on
-      // `secret`, we can assert the following on
-      // the receiver side: `assert(is_secret
-      // (join (principal_label sender)
-      // (principal_label receiver)) tr secret \/
-      // is_publishable tr payload);` 
-      is_secret (join (principal_label sender) (principal_label receiver)) tr secret
-    )
+    // The user of the communication layer can
+    // also use this function to demand specific
+    // labels from parts of the payload. These
+    // labels can then be used on the receiver
+    // side. With the following requirement on
+    // `secret`, we can assert the following on
+    // the receiver side: `assert(is_secret
+    // (join (principal_label sender)
+    // (principal_label receiver)) tr secret \/
+    // is_publishable tr payload);` 
+    is_secret (join (principal_label sender) (principal_label receiver)) tr msg.secret    
   )
 }
 #pop-options
@@ -159,21 +153,21 @@ let send_message_proof tr comm_keys_ids sender receiver state_id =
   match send_message comm_keys_ids sender receiver state_id tr with
   | (None, tr_out) -> ()
   | (Some msg_id, tr_out) -> (
-    let (Some (SenderState receiver secret), tr) = get_state sender state_id tr in
-    compute_message_proof tr sender receiver secret;
-    let payload = compute_message secret in
+    let (Some (SenderState receiver msg), tr) = get_state sender state_id tr in
     
-    let ((), tr) = trigger_event sender (SenderSendMsg sender receiver secret) tr in
+    let ((), tr) = trigger_event sender (SenderSendMsg sender receiver msg) tr in
     assert(has_communication_layer_crypto_predicates);
     assert(has_communication_layer_event_predicates comm_layer_event_preds);
-    assert(is_secret (join (principal_label sender) (principal_label receiver)) tr secret);
-    send_confidential_proof tr comm_layer_event_preds comm_keys_ids sender receiver payload;
-    let (Some msg_id, tr) = send_confidential comm_keys_ids sender receiver payload tr in
+    assert(is_secret (join (principal_label sender) (principal_label receiver)) tr msg.secret);
+    send_confidential_proof tr comm_layer_event_preds comm_keys_ids sender receiver msg;
+    let (Some msg_id, tr) = send_confidential comm_keys_ids sender receiver msg tr in
     assert(tr_out == tr);
-    assert(event_predicate_protocol tr sender (SenderSendMsg sender receiver secret));
+    assert(event_predicate_protocol tr sender (SenderSendMsg sender receiver msg));
     ()
   )
+#pop-options
 
+#push-options "--fuel 3 --ifuel 3 --z3rlimit 50"
 val receive_message_proof:
   tr:trace -> comm_keys_ids:communication_keys_sess_ids -> receiver:principal -> msg_id:timestamp ->
   Lemma
@@ -190,21 +184,25 @@ let receive_message_proof tr comm_keys_ids receiver msg_id =
   match receive_message comm_keys_ids receiver msg_id tr with
   | (None, tr_out) -> ()
   | (Some state_id, tr_out) -> (
-    let (Some payload, tr) = receive_confidential comm_keys_ids receiver msg_id tr in
-    decode_message_proof tr receiver payload;
-    let Some {secret} = decode_message payload in
-    let ((), tr) = trigger_event receiver (ReceiverReceivedMsg receiver secret payload) tr in
-    assert(event_triggered tr receiver (ReceiverReceivedMsg receiver secret payload));
-    
+    let (Some msg, tr) = receive_confidential comm_keys_ids receiver msg_id tr in
+
+    // This can be shown without an additional lemma because the post-condition
+    // of `receive_confidential_proof` contains `exists sender. is_well_formed a
+    // (is_knowable_by (comm_label sender receiver) tr) payload`
+    assert(is_knowable_by (principal_label receiver) tr msg.secret);
+
+    let ((), tr) = trigger_event receiver (ReceiverReceivedMsg receiver msg) tr in
+    assert(event_triggered tr receiver (ReceiverReceivedMsg receiver msg));
+
     // This can be shown because the
     // `comm_layer_event_preds.send_conf`
     // predicate guarantees this label of `secret`
     // on the sender side.
-    FStar.Classical.move_requires (parse_wf_lemma single_message (is_publishable tr)) payload;
-    assert(exists sender. is_secret (join (principal_label sender) (principal_label receiver)) tr secret \/
-      is_publishable tr secret);
+    assert(exists sender. is_secret (join (principal_label sender) (principal_label receiver)) tr msg.secret \/
+      is_publishable tr msg.secret);
+    
     let (state_id, tr) = new_session_id receiver tr in
-    let ((), tr) = set_state receiver state_id (ReceiverState secret payload) tr in
+    let ((), tr) = set_state receiver state_id (ReceiverState msg) tr in
     assert(tr_out == tr);
     ()
   )
