src/single_conf_and_auth_message/DY.Example.SingleConfAuthMessage.SecurityProperties.fst
@@ -3,6 +3,7 @@ module DY.Example.SingleConfAuthMessage.SecurityProperties
 open Comparse
 open DY.Core
 open DY.Lib
+open DY.Example.SingleConfAuthMessage.Protocol.Total
 open DY.Example.SingleConfAuthMessage.Protocol.Total.Proof
 open DY.Example.SingleConfAuthMessage.Protocol.Stateful
 open DY.Example.SingleConfAuthMessage.Protocol.Stateful.Proof
@@ -14,51 +15,51 @@ open DY.Example.SingleConfAuthMessage.Protocol.Stateful.Proof
 val sender_authentication:
   tr:trace -> i:timestamp ->
   sender:principal -> receiver:principal ->
-  secret:bytes ->
+  msg:single_message ->
   Lemma
   (requires
     trace_invariant tr /\
-    event_triggered_at tr i receiver (ReceiverReceivedMsg sender receiver secret)
+    event_triggered_at tr i receiver (ReceiverReceivedMsg sender receiver msg)
   )
   (ensures
-    event_triggered tr sender (SenderSendMsg sender receiver secret) \/
+    event_triggered tr sender (SenderSendMsg sender receiver msg) \/
     is_corrupt tr (long_term_key_label sender)
   )
-let sender_authentication tr i sender receiver secret = ()
+let sender_authentication tr i sender receiver msg = ()
 
 
 // Secrecy property of the secret from the sender's perspective
 val secret_secrecy_sender:
-  tr:trace -> sender:principal -> receiver:principal -> secret:bytes ->
+  tr:trace -> sender:principal -> receiver:principal -> msg:single_message ->
   Lemma
   (requires
     trace_invariant tr /\
-    attacker_knows tr secret /\
-    (exists sess_id. state_was_set tr sender sess_id (SenderState receiver secret))
+    attacker_knows tr msg.secret /\
+    (exists sess_id. state_was_set tr sender sess_id (SenderState receiver msg))
   )
   (ensures
     is_corrupt tr (principal_label sender) \/ is_corrupt tr (principal_label receiver)
   )
-let secret_secrecy_sender tr sender receiver secret =
-  attacker_only_knows_publishable_values tr secret;
+let secret_secrecy_sender tr sender receiver msg =
+  attacker_only_knows_publishable_values tr msg.secret;
   ()
 
 // Since the message is authenticated we can prove from the receiver's
 // perspective that if the attacker knows the secret, either the sender or the
 // receiver is corrupt.
 val secret_secrecy_receiver:
-  tr:trace -> sender:principal -> receiver:principal -> secret:bytes ->
+  tr:trace -> sender:principal -> receiver:principal -> msg:single_message ->
   Lemma
   (requires
     trace_invariant tr /\
-    attacker_knows tr secret /\
-    event_triggered tr receiver (ReceiverReceivedMsg sender receiver secret)
+    attacker_knows tr msg.secret /\
+    event_triggered tr receiver (ReceiverReceivedMsg sender receiver msg)
   )
   (ensures
     is_corrupt tr (principal_label sender) \/
     is_corrupt tr (principal_label receiver) \/
     is_corrupt tr (long_term_key_label sender)
   )
-let secret_secrecy_receiver tr sender receiver secret =
-  attacker_only_knows_publishable_values tr secret;
+let secret_secrecy_receiver tr sender receiver msg =
+  attacker_only_knows_publishable_values tr msg.secret;
   ()
